\newcommand{\authorinfo}{Paul Bienkowski, Hans Ole Hatzel}
\newcommand{\titleinfo}{ALA 04 (HA) zum 02.05.2013}

% PREAMBLE ===============================================================

\documentclass[a4paper,11pt]{scrartcl}
\usepackage[german,ngerman]{babel}
\usepackage[utf8]{inputenc}
\usepackage[T1]{fontenc}
\usepackage{lmodern}
\usepackage{amssymb}
\usepackage{amsmath}
\usepackage{enumerate}
\usepackage{fancyhdr}
\usepackage{pgfplots}
\usetikzlibrary{calc}

\author{\authorinfo}
\title{\titleinfo}
\date{\today}

\pagestyle{fancy}
\fancyhf{}
\fancyhead[L]{\authorinfo}
\fancyhead[R]{\titleinfo}
\fancyfoot[C]{\thepage}

\newcommand{\bra}[1]{\left(#1\right)}
\newcommand{\limnn}[2]{\lim\limits_{n \rightarrow #1}\bra{#2}}
\newcommand{\limn}[1]{\lim\limits_{n \rightarrow \infty}\bra{#1}}
\newcommand{\rowi}[1]{\sum_{i=#1}^{\infty}}
\newcommand{\row}{\rowi{0}}

\begin{document}
\maketitle
\begin{enumerate}
    \item[\textbf{1.}]
    \begin{enumerate}
        \item[a)]
        \begin{enumerate}
            \item[(i)]  \( f'(x) = 35x^4 + 9x^2 + 1 \)
            \item[(ii)] \( f'(x) = 8(3x^7 - 4x^3 + x^2 - 3x + 1)^7 \cdot (21x^6 - 12x^2 + 2x -3) \)
            \item[(iii)]\( f'(x) = (3x^4 + 2x)(\frac{x}{\sqrt{x^2+1}}) + (12x^3 + 2) \sqrt{x^2 + 1} \)
            \item[(iv)] \( f'(x) = (x^3 + 1)(\frac{4x^3+6x}{x^4+3x^2+1}) + 3x \cdot \ln\bra{x^4+3x^2+1} \)
            \item[(v)]  \( f'(x) = e^{x^3 + x^2 +1} \bra{\frac{1}{2\sqrt{x}} + 3x^2\sqrt{x} + 2x\sqrt{x}} \)
            \item[(vi)] \( f'(x) = \frac{4x^3}{2\sqrt{x^4+1}} \cdot \ln(x) + \frac{1}{x} \sqrt{x^4 + 1} \)
        \end{enumerate}

        \item[b)]
            \( q(x) = \frac{5x^2+1}{x-3} \)

            \( q'(x) = \frac{10x(x - 3) - (5x^2 + 1)}{(x-3)^2} = \frac{5x^2 - 30x - 1}{(x-3)^2} \)

            \( q''(x) = \frac{(10x - 30)(x-3)^2 - (5x^2 - 30x - 1) \cdot 2(x-3)}{(x-3)^4}
            = \frac{10 (x-3)^2 - 10x^2 + 60x + 2}{(x-3)^3} \)

            \( q'''(x) = \frac{\bra{20(x-3)-20x+60}(x-3)^3 - \bra{10(x-3)^2-10x^2+60x+2} \cdot 3(x-3)^2}{(x-3)^6}
            = -\frac{21}{(x-3)^4} \)
    \end{enumerate}

    \item[\textbf{2.}]
        \[
            \lim\limits_{x \rightarrow 6}\bra{\frac{f(x) - f(6)}{x-6}} =
            \lim\limits_{x \rightarrow 6}\bra{\frac{|3 - \frac{1}{2}x| - |3 - \frac{1}{2} \cdot 6}{x-6}} =
            \lim\limits_{x \rightarrow 6}\bra{\frac{|3 - \frac{1}{2}x|}{x-6}} = \]
        \[
            \lim\limits_{x \rightarrow 6}\bra{\sqrt{\frac{(3 - \frac{1}{2}x)^2}{(x-6)^2}}} =
            \sqrt{\lim\limits_{x \rightarrow 6}\bra{\frac{9 - 3x + \frac{1}{4}x^2}{x^2 - 2x + 36}}} =
            \sqrt{\frac{1}{4}} = \frac{1}{2}
        \]

        \begin{center}\begin{tikzpicture}[>=stealth]
            \begin{axis}[
                ymin=0,ymax=4,
                xmin=-1,xmax=8,
                x=1cm, y=1cm,
                axis x line=middle,
                axis y line=middle,
                axis line style=->,
                xlabel={$x$},
                ylabel={$y$},
                ]
                \addplot[no marks, black, -] expression[domain=-1:6,samples=4]{3-(1/2)*x} node[pos=0.65,anchor=north]{};
                \addplot[no marks, black, -] expression[domain=6:9,samples=4]{-3+(1/2)*x} node[pos=0.65,anchor=north]{};
            \end{axis}
        \end{tikzpicture}\end{center}

    \item[\textbf{3.}]
    \begin{enumerate}
        \item[a)]
    \end{enumerate}

    \item[\textbf{4.}]
    \begin{enumerate}
        \item[a)]
    \end{enumerate}
\end{enumerate}

\end{document}
